

SGD on Least Squares

Problem:

Let $\hat{L}_n(w) = \frac{1}{n} \sum_{i=1}^n (\langle w, x_i \rangle - y_i)^2$, $w \in \mathbb{R}^d$
where $x_i \in \mathbb{R}^d$, $y_i \in \mathbb{R}$ and assume $X^T X$
is invertible for $X = [x_1, \dots, x_n]^T$

The ERM is $\hat{w}_n = (X^T X)^{-1} X^T y$

We run SGD:

$$w_{t+1} = w_t - \eta_t g_t,$$

$$g_t(w_t) = 2(\langle w_t, x_{it} \rangle - y_{it}) x_{it}$$

where each i_t is chosen uniformly at

random from $\{1, \dots, n\}$ and the step
sizes satisfy

$$\sum_{t=1}^{\infty} \eta_t = \infty, \quad \sum_{t=1}^{\infty} \eta_t^2 < \infty$$

Assume $\|x_i\| \leq R \quad \forall i$

Show that $E \|w_t - \hat{w}_n\|^2 \rightarrow 0$ as $t \rightarrow \infty$

Solution:

The gradient:

$$\nabla \hat{L}_n(w) = \frac{2}{n} X^T (Xw - y) = Hw - \frac{2}{n} X^T y$$

Hessian:

$$H = \nabla^2 \hat{L}_n(w) = \frac{2}{n} \underbrace{X^T X}_{> 0}$$

$\Rightarrow H$ is positive definite > 0

Let $\mu = \lambda_{\min}(H) > 0$, $L = \lambda_{\max}(H)$

Then \hat{L}_n is μ -strongly convex and has L -Lipschitz gradient

$$\begin{aligned} & \langle \nabla \hat{L}_n(w) - \nabla \hat{L}_n(\hat{w}_n), w - \hat{w}_n \rangle \\ &= \langle H(w - \hat{w}_n), w - \hat{w}_n \rangle \\ &= (w - \hat{w}_n)^T H (w - \hat{w}_n) \geq \\ &\geq \mu \|w - \hat{w}_n\|^2 \end{aligned} \quad (1)$$

$$\begin{aligned} \|\nabla \hat{L}_n(w) - \nabla \hat{L}_n(\hat{w}_n)\| &= \|H(w - \hat{w}_n)\| \\ &\stackrel{=0}{=} \leq L \|w - \hat{w}_n\| \end{aligned} \quad (2)$$

For any w

$$E[g_+(w_t) | w_t = w]$$

$$= \frac{1}{n} \sum_{i=1}^n 2(\langle w, x_i \rangle - y_i) x_i = \nabla \hat{L}_n(w)$$

$\Rightarrow g_+$ is an unbiased estimator of the true gradient

Let $r_i = \langle \hat{w}_n, x_i \rangle - y_i$ be the residuals at the ERM

$$\begin{aligned} \|g_+(w) - g_+(\hat{w}_n)\| &= \|2\langle w - \hat{w}_n, x_{it} \rangle x_{it}\| \\ &= 2 \|x_{it}^T (w - \hat{w}_n) x_{it}\| \\ &\leq 2 \underbrace{\|x_{it}\|} \|w - \hat{w}_n\| \underbrace{\|x_{it}\|} \end{aligned}$$

$$\leq 2R^2 \|w - \hat{w}_n\|$$

Using $\|a+b\|^2 \leq 2\|a\|^2 + 2\|b\|^2$

$$\underline{E \|g_+(w)\|^2} = E \left\| \underbrace{g_+(w) - g_+(\hat{w}_n)}_a + \underbrace{g_+(\hat{w}_n)}_b \right\|^2$$

$$\leq 2 E \|g_+(w) - g_+(\hat{w}_n)\|^2 + 2 E \|g_+(\hat{w}_n)\|^2$$
$$4R^4 \|w - \hat{w}_n\|^2$$

(3)

$C :=$

$$\leq \underbrace{8R^4 \|w - \hat{w}_n\|^2}_{< \infty} + \underbrace{\frac{2}{n} \sum_{i=1}^n 4\tau_i^2 R^2}_{2^2 \text{ residual def}} \leftarrow \text{bound on } \|x_i\|^2$$

$$E\langle A, B \rangle$$

$$E\langle \mathbb{E}[A], E[B] \rangle$$

Expand one SGD step

$$\begin{aligned} \|w_{t+1} - \hat{w}_n\|^2 &= \|w_t - \hat{w}_n - \eta_t g_t\|^2 \\ &= \|w_t - \hat{w}_n\|^2 - 2\eta_t \langle w_t - \hat{w}_n, g_t \rangle + \eta_t^2 \|g_t\|^2 \\ \Rightarrow E\|w_{t+1} - \hat{w}_n\|^2 &= E\|w_t - \hat{w}_n\|^2 - 2\eta_t E\langle w_t - \hat{w}_n, g_t \rangle + \eta_t^2 E\|g_t\|^2 \end{aligned}$$

$$E\langle w_t - \hat{w}_n, E[g_t] \rangle$$

By (1), $E\langle w_t - \hat{w}_n, g_t(w_t) \rangle \geq \mu \|w_t - \hat{w}_n\|^2$

$$E\|w_{t+1} - \hat{w}_n\|^2 = (1 - 2\mu\eta_t + \eta_t^2 \cdot 8R^4) E\|w_t - \hat{w}_n\|^2 + C\eta_t^2$$

We know $\eta_t \rightarrow 0$ as $t \rightarrow \infty$

$\exists N$ s.t. $\forall t \geq N$

$$2\mu\eta_t - 8R^4\eta_t^2 \geq \mu\eta_t \quad (\eta_N \leq \frac{\mu}{8R^4})$$

(4)

$$\Rightarrow E \|w_{t+1} - \hat{w}_n\|^2 \leq (1 - \mu \eta_t^2) \underbrace{E \|w_t - \hat{w}_n\|^2}_{a_t} + C \eta_t^2$$

$$\forall t \geq N \quad a_{t+1} \leq (1 - \mu \eta_t^2) a_t + C \eta_t^2$$

$$a_t \leq (1 - \mu \eta_{t-1}^2) a_{t-1} + C \eta_{t-1}^2$$

$$a_{t+1} \leq (1 - \mu \eta_t^2) (1 - \mu \eta_{t-1}^2) a_{t-1} \\ + (1 - \mu \eta_t^2) C \eta_{t-1}^2 + C \eta_t^2$$

$$\leq \dots$$

$$\leq a_N \prod_{k=N}^t (1 - \mu \eta_k^2) + \\ C \sum_{k=N}^t \eta_k^2 \prod_{j=k+1}^t (1 - \mu \eta_j^2)$$

$$\text{where } \prod_{j=t+1}^t (1 - \mu \eta_j^2) = 1$$

$$M = \max_{i=1, \dots, N} \frac{a_i}{\eta_i^2} \rightarrow 0 \text{ as } t \rightarrow \infty$$

$$a_{t+1} \leq M \left[\prod_{k=N}^t (1 - \mu \eta_k^2) + \sum_{k=N}^t \eta_k^2 \prod_{j=k+1}^t (1 - \mu \eta_j^2) \right] \rightarrow 0$$

$$\log(1-x) \leq -x \rightarrow 0$$

$$\left(\begin{aligned} \log \prod (1 - \mu \eta_k^2) &= \sum \log(1 - \mu \eta_k^2) \\ &\leq \sum -\mu \eta_k^2 \leq -\infty \end{aligned} \right)$$

$$\Rightarrow E \|w_{t+1} - \hat{w}_n\|^2 \rightarrow 0 \text{ as } t \rightarrow \infty$$